theories/L/Functions/EqBool.v
@@ -1,4 +1,6 @@
 From Undecidability.L Require Import L Tactics.LTactics LBool.
+(*From Undecidability.L.Complexity Require Import Monotonic UpToC.*)
+
 
 Class eqbClass X (eqb : X -> X -> bool): Type := 
   _eqb_spec : forall (x y:X), reflect (x=y) (eqb x y).
@@ -34,8 +36,8 @@ Qed.
 
 Class eqbCompT X {R:registered X} eqb {H:eqbClass (X:=X) eqb} :=
   { c__eqbComp :nat;
-    eqbTime x y:= min (size (enc x)) (size (enc y))* c__eqbComp;
-    comp_eqb : computableTime' eqb (fun x _ =>(5,fun y _ => (eqbTime x y,tt)))
+    eqbTime x y:= min x y* c__eqbComp;
+    comp_eqb : computableTime' eqb (fun x _ =>(5,fun y _ => (eqbTime (size (enc x)) (size (enc y)),tt)))
   }.
 Arguments eqbCompT _ {_ _ _}.
 Arguments c__eqbComp _ {_ _ _ _}.
@@ -53,3 +55,26 @@ Proof.
   [c]:exact 3.
   all:unfold c;try lia.
 Qed.
+
+Lemma eqbTime_le_l X (R : registered X) (eqb : X -> X -> bool) (H : eqbClass eqb)
+      (eqbCompT : eqbCompT X) x n':
+  eqbTime x n' <= x * c__eqbComp X.
+Proof.
+  unfold eqbTime. rewrite Nat.le_min_l. easy.
+Qed.
+
+Lemma eqbTime_le_r X (R : registered X) (eqb : X -> X -> bool) (H : eqbClass eqb)
+      (eqbCompT : eqbCompT X) x n':
+  eqbTime n' x <= x * c__eqbComp X.
+Proof.
+  unfold eqbTime. rewrite Nat.le_min_r. easy.
+Qed.
+
+(*
+Lemma eqbTime_upToC X {R:registered X} eqb {H:eqbClass (X:=X) eqb} {_:eqbCompT X}:
+  eqbTime (X:=X) <=c (fun (x y:nat) => min x y).
+Proof.
+  unfold eqbTime. hnf.
+  exists (c__eqbComp X). unfold leHO;repeat intro; cbn;nia.
+Qed.
+*)
