theories/L/TM/TMflatComp.v
@@ -1,13 +1,123 @@
 From Undecidability.TM Require Import TM.
-From Undecidability.L.TM Require Import TMflat TMflatEnc TMflatFun TMEncoding TapeDecode TMunflatten TapeFuns.
+From Undecidability.L.TM Require Import TMflat TMflatEnc TMflatFun TMEncoding TMunflatten TapeFuns.
 From Undecidability.L.Datatypes Require Import LNat LProd Lists LOptions.
  
-From Undecidability.L.Complexity Require Import NP LinTimeDecodable.
+From Undecidability.L.Complexity Require Import ONotation Monotonic.
 From Undecidability.L Require Import Tactics.LTactics Functions.Decoding TMflatFun.
 From Undecidability Require Import L.Functions.EqBool.
 
+Definition haltConfFlat_time (c : nat) := 20 * c + 21.
+
+Instance term_haltConfFlat : computableTime' haltConfFlat (fun f _ => (1, fun c _ => (haltConfFlat_time (fst c),tt))).
+Proof.
+  extract. unfold haltConfFlat_time. solverec.
+Qed.
+
+
+Definition zipWith_time {X Y} (fT : X -> Y -> nat) (xs:list X) (ys:list Y) := sumn (zipWith (fun x y => fT x y + 18) xs ys) + 9.
+Instance term_zipWith A B C `{registered A} `{registered B} `{registered C}:
+  computableTime' (@zipWith A B C) (fun _ fT => (1, fun xs _ => (5,fun ys _ => (zipWith_time (callTime2 fT) xs ys, tt)))).
+Proof.
+  extract. unfold zipWith_time. solverec.
+Qed.
+
+Lemma zipWith_time_const {X Y} c (xs:list X) (ys : list Y):
+  zipWith_time (fun _ _ => c) xs ys = min (length xs) (length ys) * (c + 18) + 9.
+Proof.
+  induction xs in ys |-*;cbn. nia. destruct ys;cbn. nia.
+  unfold zipWith_time in *.
+  specialize (IHxs ys). nia.
+Qed.
+
+(*MOVE*)
+Instance term_repeat A `{registered A}: computableTime' (@repeat A) (fun _ _ => (5, fun n _ => (n * 12 + 4,tt))).
+Proof.
+  extract. solverec.
+Qed.
+
+From Undecidability.L Require Import Functions.FinTypeLookup.
+Definition stepFlat_time (f : nat) (c:mconfigFlat) := 153 * (| snd c |) + f * size (enc (fst c, map (current (sig:=nat)) (snd c))) * c__eqbComp (nat * list (option nat)) + 24 * f + 89.
+
+Instance term_stepFlat : computableTime' stepFlat (fun f _ => (1, fun c _ => (stepFlat_time (length f) c,tt))).
+Proof.
+  unfold stepFlat.
+  extract.
+  solverec.
+  rewrite map_time_const,zipWith_time_const, lookupTime_leq.
+  rewrite Nat.le_min_l.
+  unfold stepFlat_time.
+  nia.
+Qed.
+
+Definition loopMflat_time M c k := loopTime (stepFlat (trans M)) (fun (c0 : mconfigFlat) (_ : unit) => (stepFlat_time (| trans M |) c0, tt)) (haltConfFlat (halt M))
+    (fun (c0 : nat * list (tape nat)) (_ : unit) => (haltConfFlat_time (fst c0), tt)) c k.
+
+
+Instance term_loopMflat : computableTime' loopMflat (fun M _ => (23,fun c  _ => (5, fun k _ => (loopMflat_time M c k,tt)))).
+Proof.
+  unfold loopMflat,loopMflat_time.
+  extract. solverec.
+Qed.
+
+Lemma haltConfFlat_time_le s states:
+  s <= states -> haltConfFlat_time s <= haltConfFlat_time states.
+Proof.
+  unfold haltConfFlat_time. lia.
+Qed.
+
+Definition stepFlat_timeNice n st sig f :=
+  153 * n + f * (st * 4 + 4 + (n * (4 * sig + 19) + 4) + 4) * c__eqbComp (nat * list (option nat)) + 24 * f + 89.
+
+Lemma stepFlat_time_nice M f c:
+  validFlatConf M c ->
+  stepFlat_time f c <= stepFlat_timeNice M.(tapes) M.(states) M.(sig) f.
+Proof.
+  intros H.
+  unfold stepFlat_time.
+  destruct c as (s,t);cbn [fst snd]. destruct H as (eqt&?&?).
+  rewrite size_prod;cbn [fst snd].
+  rewrite size_nat_enc.
+  rewrite size_list. rewrite sumn_le_bound with (c:=4*M.(sig) + 19).
+  2:{ rewrite map_map. intros ? (?&<-&?)%in_map_iff. rewrite size_option.
+      rewrite Forall_forall in H. apply H in H1.
+      destruct x;cbn. 1-3:lia. rewrite size_nat_enc. destruct (H1 n).
+      cbn;eauto. all:nia. }
+  rewrite !map_length.
+  rewrite eqt. unfold stepFlat_timeNice. nia.
+Qed.
+
+Definition loopMflat_timeNice M k := 
+  k * (stepFlat_timeNice M.(tapes) M.(states) M.(sig) (length M.(trans))  + haltConfFlat_time M.(states) + 13) + haltConfFlat_time M.(states) + 7.
+
+Lemma validFlatConf_step M c c' :
+  validFlatTM M -> validFlatConf M c -> stepFlat (M.(trans)) c = c' ->  validFlatConf M c'.
+Admitted. 
+
+Lemma loopMflat_time_nice M c k:
+  validFlatTM M  -> validFlatConf M c
+  -> loopMflat_time M c k <= loopMflat_timeNice M k.
+Proof.
+  intros HM Hc.
+  unfold loopMflat_time.
+  induction k in c,Hc|-*;
+  destruct c as (s,t); inversion Hc as (?&?&?);cbn [fst snd].
+  all:cbn [loopTime fst snd].
+  {rewrite haltConfFlat_time_le with (states:=M.(states)). all:unfold loopMflat_timeNice; try nia. }
+  destruct stepFlat as (s',t') eqn:eq.
+  assert (validFlatConf M (s', t')) by eauto using validFlatConf_step.  
+  setoid_rewrite IHk. 2:easy. 
+  rewrite haltConfFlat_time_le with (states:=M.(states)). 2:nia.
+  rewrite (stepFlat_time_nice (M:=M)). 2:easy. 
+  unfold loopMflat_timeNice; nia.
+Qed.
+
+
+
+Definition sizeOfmTapesFlat_time sig (t : list (tape sig))
+  := sumn (map (@sizeOfTape _) t) * 55 + length t * 58 + 8.
+
 Instance term_sizeOfmTapesFlat sig {H:registered sig}:
-  computableTime' (@sizeOfmTapesFlat sig) (fun t _ => (sumn (map (@sizeOfTape _) t) * 55 + length t * 58 + 8,tt)).
+  computableTime' (@sizeOfmTapesFlat sig) (fun t _ => (sizeOfmTapesFlat_time t,tt)).
 Proof.
   assert (H' : extEq
                  (fix sizeOfmTapesFlat (ts : list (tape sig)) : nat :=
@@ -19,7 +129,19 @@ Proof.
   cbn [extEq] in H'.
   
   eapply computableTimeExt. exact H'.
-  extract. solverec. 
+  extract. unfold sizeOfmTapesFlat_time. solverec. 
+Qed.
+
+Definition sizeOfmTapesFlat_timeSize n := n * 57.
+Lemma sizeOfmTapesFlat_timeBySize {sig} `{registered sig} (t:list (tape sig)) :
+  sizeOfmTapesFlat_time t <= sizeOfmTapesFlat_timeSize (size (enc t)).
+Proof.
+  unfold sizeOfmTapesFlat_time,sizeOfmTapesFlat_timeSize.
+  rewrite size_list.
+  induction t.
+  all:cbn [map sumn length].
+  now nia.
+  rewrite sizeOfTape_by_size. nia.
 Qed.
 
 
@@ -29,10 +151,26 @@ Definition allSameEntry_helper {X Y} eqbX eqbY `{_:eqbClass (X:=X) eqbX} `{eqbCl
 Instance term_allSameEntry_helper {X Y} {HX:registered X} {HY:registered Y}
          `{eqbCompT X (R:=HX)} `{eqbCompT Y (R:=HY)}
   :
-    computableTime' (@allSameEntry_helper X Y _ _ _ _) (fun x _ => (1,fun y _ =>(1,fun xy _ => (eqbTime x (fst xy) + eqbTime y (snd xy) + 18,tt)))).
+    computableTime' (@allSameEntry_helper X Y _ _ _ _)
+                    (fun x _ => (1,fun y _ =>(1,fun xy _ => (eqbTime (X:=X) (size (enc x)) (size (enc (fst xy))) + eqbTime (X:=Y) (size (enc y)) (size (enc (snd xy))) + 18,tt)))).
 Proof.
   unfold allSameEntry_helper. unfold implb. extract. solverec.
 Qed.
+
+Definition allSameEntry_time X Y {HX:registered X} {HY:registered Y}
+           `{eqbCompT X (R:=HX)} `{eqbCompT Y (R:=HY)} l x y :=
+  l * (x*c__eqbComp X + y* c__eqbComp Y + 42) + 12.
+
+Arguments allSameEntry_time : clear implicits.
+Arguments allSameEntry_time _ _ {_ _ _ _ _ _ _ _} _ _.
+
+
+Lemma allSameEntry_time_le X Y {HX:registered X} {HY:registered Y}
+           `{eqbCompT X (R:=HX)} `{eqbCompT Y (R:=HY)} l l' x x' y y' :
+  l <= l' -> x <= x' -> y <= y'
+  -> allSameEntry_time X Y l x y <= allSameEntry_time X Y l' x' y'.
+Proof. unfold allSameEntry_time. intros -> -> ->. nia. Qed.
+
 
 Instance term_allSameEntry X Y {HX:registered X} {HY:registered Y}
          `{eqbCompT X (R:=HX)} `{eqbCompT Y (R:=HY)}:
@@ -40,7 +178,7 @@ Instance term_allSameEntry X Y {HX:registered X} {HY:registered Y}
                     fun x _ => (1,
                              fun y _ => (1,
                                       fun f _ =>(
-                                          length f * (size (enc x)*c__eqbComp X + size (enc y)* c__eqbComp Y + 42) + 12,tt)))).
+                                          allSameEntry_time X Y (length f) (size (enc x)) (size (enc y)),tt)))).
 
 Proof.
   unfold allSameEntry.
@@ -49,23 +187,40 @@ Proof.
   extract.
   recRel_prettify2. 1-2:easy.
   clear.
-  rename x1 into f.
+  rename x1 into f. unfold allSameEntry_time.
   
   change 12 with (8+4) at 3. rewrite !Nat.add_assoc. eapply plus_le_compat_r.
   
   induction f as [ | [x' y'] f].
   { easy. }
-  cbn - [plus mult] . unfold eqbTime. rewrite IHf.
+  cbn - [plus mult] . rewrite IHf.
+  do 2 rewrite eqbTime_le_l.  clear. ring_simplify. 
   nia.
 Qed.
 
+(*MOVE*)
+Lemma size_list_cons (X : Type) (H : registered X) x (l : list X):
+  size (enc (x::l)) = size (enc x) + size (enc l) + 5.
+Proof.
+  rewrite !size_list. cbn. lia.
+Qed.
+
+Definition isInjFinfuncTable_time X Y {HX:registered X} {HY:registered Y}
+           `{eqbCompT X (R:=HX)} `{eqbCompT Y (R:=HY)} l sf :=
+  l * (allSameEntry_time X Y l sf sf + 21) + 8.
+
 Instance term_isInjFinfuncTable X Y {HX:registered X} {HY:registered Y}
          `{eqbCompT X (R:=HX)} `{eqbCompT Y (R:=HY)}:
-  computableTime' (@isInjFinfuncTable X Y _ _ _ _) (fun f _ => (length f * (size (enc f) * (c__eqbComp X + c__eqbComp Y + 5)) + 8,tt)).
+  computableTime' (@isInjFinfuncTable X Y _ _ _ _) (fun f _ => (isInjFinfuncTable_time (X:=X) (Y:=Y) (length f) (size (enc f)),tt)).
 Proof.
-  unfold isInjFinfuncTable. cbn. extract.
+  unfold isInjFinfuncTable. cbn. extract. unfold isInjFinfuncTable_time.
   solverec. subst.
-  cbn [length]. rewrite !size_list. cbn [map sumn]. rewrite !size_prod. cbn [fst snd]. nia.
+  rewrite size_list_cons.
+  setoid_rewrite <- allSameEntry_time_le with (l:=length l) (x:=(size (enc x))) (y:=size(enc y)) at 4.
+  2:nia.
+  2,3:now rewrite size_prod;cbn [fst snd];nia.
+  setoid_rewrite <- allSameEntry_time_le with (l:=length l) (x:=(size (enc l))) (y:=size(enc l)) at 3.
+  all:try nia.
 Qed.
 
 Definition isBoundRead sig := fun a : option nat => match a with
@@ -145,14 +300,151 @@ Proof.
   all:ring_simplify. zify. clear; nia.
 Qed.
 
+Definition time_isValidFlatTrans lf sf := isInjFinfuncTable_time (X:=nat * list (option nat)) (Y:=(nat * list (option nat * move))) lf sf + sf * (c__eqbComp nat + 8) + 9.
+
 Instance term_isValidFlatTrans:
-  computableTime' (isValidFlatTrans) (fun _ _ => (1,
-                                               fun _ _ => (1,
-                                                        fun states_ _ => (1,
-                                                                       fun f _ => 
-                                                                         (size (enc f)* (8+c__eqbComp nat + length f * (c__eqbComp (nat*(list (option nat)))
-                                                                                                                    + c__eqbComp (nat*(list (option nat * move))) + 5))+ 17,tt))))).
+  computableTime' (isValidFlatTrans)
+                  (fun _ _ => (1,
+                   fun _ _ => (1,
+                   fun _ _ => (1,
+                   fun f _ => 
+                    (time_isValidFlatTrans (length f)(size (enc f)),tt))))).
 Proof.
   unfold isInjFinfuncTable. cbn. extract.
+  solverec. unfold time_isValidFlatTrans. nia.
+Qed.
+
+Definition isValidFlatTM_time lf sf st:= time_isValidFlatTrans lf sf+ st*14 + 77.
+
+Instance term_isValidFlatTM : computableTime' isValidFlatTM (fun M _ => (isValidFlatTM_time (length (trans M)) (size (enc (trans M))) (states M),tt)).
+Proof.
+  unfold isValidFlatTM. unfold Nat.ltb.
+  extract. unfold isValidFlatTM_time. solverec.
+Qed.
+
+Definition  isValidFlatTape_time (sig:nat) (t:nat) :=
+  t * (sig * 14 + 29 + 44) + 37.
+
+Lemma isValidFlatTape_time_le sig t t' :
+  t <= t' -> isValidFlatTape_time sig t <= isValidFlatTape_time sig t'.
+Proof. unfold isValidFlatTape_time. intros ->. nia. Qed. 
+
+
+Instance term_isValidFlatTape : computableTime' isValidFlatTape
+            (fun sig _ => (1, fun t _ => (isValidFlatTape_time sig (sizeOfTape t),tt))).
+Proof.
+  pose (f x y:= Nat.ltb y x).
+  unfold isValidFlatTape.
+  refine (_:computableTime' (fun (sig : nat) (t : tape nat) => forallb (f sig) (tapeToList t)) _).
+  
+  assert (computableTime' f (fun x _ =>(1, fun y _ => (Init.Nat.min y x * 14 + 29, tt)))).
+  { unfold f,Init.Nat.ltb. extract. solverec. }
+
+  extract. solverec.
+  evar (c:nat).
+  rewrite forallb_time_eq,sumn_le_bound with (c:=c).
+  2:{ intros ? (?&<-&?)%in_map_iff. rewrite Nat.le_min_r. unfold c;reflexivity. }
+  rewrite map_length. fold (sizeOfTape x0).
+  unfold isValidFlatTape_time,c. lia.
+Qed.
+
+
+(*MOVE*)
+Definition lengthEq A :=
+  fix f (t:list A) n :=
+    match n,t with
+      0,nil => true
+    | (S n), _::t => f t n
+    | _,_ => false
+    end.
+Lemma lengthEq_spec A (t:list A) n:
+| t | =? n = lengthEq t n.
+Proof.
+  induction n in t|-*;destruct t;now cbn.
+Qed.
+Definition lengthEq_time k := k * 15 + 9.
+Instance term_lengthEq A `{registered A} : computableTime' (lengthEq (A:=A)) (fun l _ => (5, fun n _ => (lengthEq_time (min (length l) n),tt))).
+Proof.
+  extract. unfold lengthEq_time. solverec.
+Qed.
+
+Definition  isValidFlatTapes_time (sig lt mt :nat) := lt*(isValidFlatTape_time sig mt + 30) + 28.
+
+
+Instance term_isValidFlatTapes : computableTime' isValidFlatTapes (fun sig _ => (1, fun n _ => (1,fun t _ => (isValidFlatTapes_time sig n (sizeOfmTapesFlat t),tt)))).
+Proof.
+  unfold isValidFlatTapes.
+  eapply computableTimeExt with (x:= fun sig n t => if lengthEq t n then forallb (isValidFlatTape sig) t else false).
+  {intros ? ? ?;hnf. now rewrite lengthEq_spec. }
+  extract. unfold isValidFlatTapes_time,lengthEq_time.
   solverec.
+  rewrite <- lengthEq_spec in H. apply beq_nat_true in H. subst.
+  evar (c:nat).
+  rename x1 into t.
+  rewrite forallb_time_eq,sumn_le_bound with (c:=c).
+  2:{ intros ? (?&<-&?)%in_map_iff.
+      rewrite isValidFlatTape_time_le with (t':=sizeOfmTapesFlat t).
+      1:now unfold c;reflexivity.
+      clear - H. induction t;inv H. all:now cbn.
+  }
+  rewrite map_length. unfold c. nia.
+Qed.
+
+Definition execFlatTM_time (M:TM) (t:nat) (k:nat) :=
+ isValidFlatTM_time (length M.(trans)) (size (enc M.(trans))) M.(states) + isValidFlatTapes_time M.(sig) M.(tapes) t + loopMflat_timeNice M k + 66 .
+
+Instance term_execFlatTM: computableTime' execFlatTM (fun M _ => (1,fun t _ => (1,fun k _ => (execFlatTM_time M (sizeOfmTapesFlat t) k,tt)))).
+Proof.
+  extract. unfold execFlatTM_time. recRel_prettify.
+  intros M _. split. easy.
+  intros t _. split. easy.
+  intros k _. split. 2:now repeat destruct _.
+  destruct (isValidFlatTM_spec M). 2:nia.
+  destruct isValidFlatTapes eqn:Ht. 2:nia.
+  rewrite loopMflat_time_nice.
+  -nia.
+  -easy.
+  -unfold isValidFlatTapes in Ht.  hnf.
+   destruct (Nat.eqb_spec (length t) (tapes M)). 2:easy.
+   split. easy.
+   split.
+   +apply Forall_forall. rewrite forallb_forall in Ht. intros ? H'. specialize (Ht _ H'). now destruct (isValidFlatTape_spec (sig M) x).
+   +destruct v. easy.
+Qed.
+
+Lemma execFlat_poly : {f : nat -> nat & (forall M t k, execFlatTM_time M t k <= f (size (enc M) +t + k)) /\ inOPoly f /\ monotonic f}.
+Proof.
+  unfold execFlatTM_time,isValidFlatTM_time,time_isValidFlatTrans,isInjFinfuncTable_time,allSameEntry_time,loopMflat_timeNice,haltConfFlat_time,isValidFlatTapes_time,isValidFlatTape_time,stepFlat_timeNice.
+  eexists (fun x => _). split.
+  {
+    intros M t k.
+    remember ( (size (enc M) + t + k)) as x.
+    assert (Hf : (size (enc (trans M)) <= x)).
+    { subst x. rewrite size_TM. destruct M. cbn. lia. }
+    rewrite Hf. 
+
+    assert ( Hlt : | trans M | <= x).
+    { rewrite <- Hf. rewrite size_list_enc_r. lia. }
+    rewrite Hlt.
+
+    assert (Hn : tapes M <= x).
+    { subst x. rewrite size_TM. destruct M. cbn. rewrite size_nat_enc_r with (n:=tapes) at 1. lia. }
+    rewrite Hn.
+
+    assert (Hst : states M <= x).
+    { subst x. rewrite size_TM. destruct M. cbn. rewrite size_nat_enc_r with (n:=states) at 1. lia. }
+    rewrite Hst.
+
+    assert (Hsig : sig M <= x).
+    { subst x. rewrite size_TM. destruct M. cbn. rewrite size_nat_enc_r with (n:=sig) at 1. lia. }
+    rewrite Hsig.
+    
+    assert (Ht : t <= x) by lia.
+    rewrite Ht.
+
+    assert (Hk : k <= x) by lia.
+    rewrite Hk. 
+    clear. reflexivity.
+  }
+  split. all:smpl_inO.
 Qed.
