theories/L/TM/TapeFuns.v
@@ -65,11 +65,44 @@ Section fix_sig.
       extract. unfold sizeOfTape. solverec.
     Qed.
 
+    Global Instance term_current: computableTime' ((current (sig:=sig))) (fun _ _ => (10,tt)).
+    Proof.
+      extract.
+      solverec.
+    Qed.
+
+    Global Instance term_current_chars n: computableTime' (current_chars (sig:=sig) (n:=n))  (fun _ _ => (n * 22 +12,tt)).
+    Proof.
+      extract.
+      solverec.
+      rewrite map_time_const,to_list_length.  omega.
+    Qed.
+
+    Global Instance term_doAct: computableTime' (doAct (sig:=sig)) (fun _ _ => (1,fun _ _ => (89,tt))).
+    Proof.
+      extract.
+      solverec.
+    Qed.
+
 
   End reg_tapes.
 End fix_sig.
 
+Fixpoint loopTime {X} `{registered X} f (fT: timeComplexity (X -> X)) (p: X -> bool) (pT : timeComplexity (X -> bool)) (a:X) k :=
+  fst (pT a tt) +
+  match k with
+    0 => 7
+  |  S k =>
+     fst (fT a tt) + 13 + loopTime f fT p pT (f a) k
+  end.
 
+Instance term_loop A `{registered A} :
+  computableTime' (@loop A)
+                 (fun f fT => (1,fun p pT => (1,fun a _ => (5,fun k _ =>(loopTime f fT p pT a k,tt))))).
+Proof.
+  extract.
+  solverec.
+Qed.
 
 
 
