theories/L/Functions/Subst.v
@@ -2,13 +2,12 @@ From Undecidability.L Require Import Tactics.LTactics Datatypes.LNat Functions.E
 (** ** Extracted substitution on terms *)
 
 Instance term_substT :
-  computableTime' subst (fun s _ => (5, (fun n _ => (1, (fun t _ => ( (* n * (cnst 0+15) * size s + *) (size s) * (size s + c__eqbComp nat * 4 + 20), tt)))))).
+  computableTime' subst (fun s _ => (5, (fun n _ => (1, (fun t _ => ( (size s) * (size s + c__eqbComp nat * 4 + 20), tt)))))).
 Proof.
   unfold subst. change Nat.eqb with (EqBool.eqb (X:=nat)).
-  extract.
+  extract. unfold eqbTime.
 
   recRel_prettify2. all:unfold eqbTime; cbn [fst snd size].
   all:try rewrite !size_nat_enc.
-  all:try rewrite Nat.le_min_l.
-  all:ring_simplify. all:try nia.
+  all:try nia.
 Qed.
